consistency.thy
@@ -542,6 +542,12 @@ apply (auto dest: transD)
   
 
 
+lemma happensBefore_irrefl:
+assumes wf: "state_wellFormed S"
+shows "irrefl (happensBefore S)"
+using assms  apply (induct rule: wellFormed_induct) 
+  apply (auto simp add: initialState_def step_simps_all irreflI)
+  by (smt Un_iff irrefl_def mem_Sigma_iff singletonD wellFormed_visibleCallsSubsetCalls2)
 
 
 
