topological_sort.thy
@@ -1,0 +1,183 @@
+theory topological_sort
+  imports Main "HOL-Library.Multiset"
+    "fuzzyrule.fuzzyrule"
+begin
+
+definition sorted_by where
+"sorted_by rel xs \<equiv> \<forall>i j. i<j \<longrightarrow> j<length xs \<longrightarrow> (xs!j,xs!i)\<notin>rel"
+
+lemma sorted_by_empty:
+"sorted_by R []"
+  by (auto simp add: sorted_by_def)
+
+lemma sorted_by_single:
+"sorted_by R [x]"
+  by (auto simp add: sorted_by_def)
+
+lemma sorted_by_prepend_smallest:
+  assumes "\<forall>y\<in>set xs. (y,x)\<notin>R"
+    and "sorted_by R xs"
+  shows "sorted_by R (x#xs)"
+  using assms by (auto simp add: sorted_by_def nth_Cons split: nat.splits)
+
+lemma sorted_by_sublist_left:
+  assumes a: "sorted_by R (xs@ys)"
+  shows "sorted_by R xs"
+  using a by (auto simp add: sorted_by_def nth_append split: if_splits)
+
+lemma sorted_by_sublist_right:
+  assumes a: "sorted_by R (xs@ys)"
+  shows "sorted_by R ys"
+  using a by (auto simp add: sorted_by_def nth_append split: if_splits,
+      metis add.commute add_diff_cancel_left' add_less_cancel_right add_less_same_cancel1 not_less_zero)
+
+lemma sorted_by_append:
+  assumes "sorted_by R (xs @ ys)"
+      and c1: "x \<in> set xs"
+      and c2: "y \<in> set ys"
+    shows "(y, x) \<notin> R"
+  using assms apply (auto simp add: sorted_by_def nth_append in_set_conv_nth split: if_splits)
+  by (smt add_diff_cancel_left' add_diff_cancel_right' diff_le_self less_diff_conv less_le_trans not_add_less2)
+
+
+lemma sorted_by_append_iff:
+  shows "sorted_by R (xs@ys) \<longleftrightarrow> (sorted_by R xs \<and> sorted_by R ys \<and> (\<forall>x\<in>set xs. \<forall>y\<in>set ys. (y,x)\<notin>R))"
+proof auto
+  show "sorted_by R (xs @ ys) \<Longrightarrow> sorted_by R xs"
+    using sorted_by_sublist_left by blast
+  show "sorted_by R (xs @ ys) \<Longrightarrow> sorted_by R ys"
+    using sorted_by_sublist_right by blast
+
+  show "False"
+    if c0: "sorted_by R (xs @ ys)"
+      and c1: "x \<in> set xs"
+      and c2: "y \<in> set ys"
+      and c3: "(y, x) \<in> R"
+    for  x y
+    by (meson c0 c1 c2 c3 sorted_by_append)
+
+
+  show "sorted_by R (xs @ ys)"
+    if c0: "sorted_by R xs"
+      and c1: "sorted_by R ys"
+      and c2: "\<forall>x\<in>set xs. \<forall>y\<in>set ys. (y, x) \<notin> R"
+    apply (auto simp add: sorted_by_def nth_append)
+    using c0 sorted_by_def apply blast
+    apply (simp add: c2)
+    by (metis add_diff_inverse_nat c1 dual_order.strict_trans nat_add_left_cancel_less sorted_by_def)
+qed
+
+lemma sorted_by_cons_iff:
+  shows "sorted_by R (x#xs) \<longleftrightarrow> (sorted_by R xs \<and> (\<forall>y\<in>set xs. (y,x)\<notin>R))"
+  using sorted_by_append_iff[where R=R and xs="[x]" and ys="xs"]
+  by (auto simp add: sorted_by_single)
+
+
+fun top_sort where
+  "top_sort R [] = []"
+| "top_sort R (x#xs) = (
+    let (greater, not_greater) = partition (\<lambda>y. R x y) xs in
+    top_sort R not_greater @ x # top_sort R greater)"
+
+value "top_sort (\<subset>) [{1,2,3}, {1}, {1}, {2,3,4}, {2}, {1,3::int}, {}]"
+
+lemma top_sort_mset[simp]:
+"mset (top_sort R xs) = mset xs"
+proof (induct R xs rule: top_sort.induct)
+  case (1 R)
+  show "mset (top_sort R []) = mset [] "
+    by simp
+next
+  case (2 R x xs)
+  show " mset (top_sort R (x # xs)) = mset (x # xs)"
+    using 2 by auto
+qed
+
+lemma top_sort_set[simp]:
+"set (top_sort R xs) = set xs"
+  by (metis set_mset_mset top_sort_mset)
+
+
+lemma top_sort_sorts_irrefl:
+  assumes trans: "trans {(x,y). R x y}"
+    and irrefl: "irrefl {(x,y). R x y}"
+  shows "sorted_by {(x,y). R x y} (top_sort R xs)"
+using trans irrefl proof (induct R xs rule: top_sort.induct)
+case (1 R)
+  then show ?case 
+    by (auto simp add: sorted_by_empty)
+next
+  case (2 R x xs)
+  show ?case 
+  proof (auto simp add: sorted_by_append_iff sorted_by_cons_iff)
+    show "sorted_by {(x, y). R x y} (top_sort R (filter (Not \<circ> R x) xs))"
+      by (simp add: 2)
+    show "sorted_by {(x, y). R x y} (top_sort R (filter (R x) xs))"
+      by (simp add: 2)
+    show "\<And>y. \<lbrakk>y \<in> set xs; R x y; R y x\<rbrakk> \<Longrightarrow> False"
+      by (metis "2.prems"(1) "2.prems"(2) case_prodI irrefl_def mem_Collect_eq trans_def)
+    show "\<And>xa y. \<lbrakk>xa \<in> set xs; \<not> R x xa; y \<in> set xs; R x y; R y xa\<rbrakk> \<Longrightarrow> False"
+      by (smt "2.prems"(1) case_prodD case_prodI mem_Collect_eq transE)
+  qed
+qed
+
+lemma top_sort_sorts_distinct:
+  assumes trans: "trans {(x,y). R x y}"
+    and irrefl: "\<And>x y. x\<in>set xs \<Longrightarrow> y\<in>set xs \<Longrightarrow> R x y \<Longrightarrow> x\<noteq>y \<Longrightarrow> \<not>R y x"
+    and distinct: "distinct xs"
+  shows "sorted_by {(x,y). R x y} (top_sort R xs)"
+using trans irrefl distinct proof (induct R xs rule: top_sort.induct)
+case (1 R)
+  then show ?case 
+    by (auto simp add: sorted_by_empty)
+next
+  case (2 R x xs)
+  have irrefl: "\<And>x y. x\<in>set xs \<Longrightarrow> y\<in>set xs \<Longrightarrow> R x y \<Longrightarrow> x\<noteq>y \<Longrightarrow> \<not>R y x"
+    by (simp add: "2.prems"(2))
+
+  show ?case 
+  proof (auto simp add: sorted_by_append_iff sorted_by_cons_iff)
+    show "sorted_by {(x, y). R x y} (top_sort R (filter (Not \<circ> R x) xs))"
+      by (rule 2, insert "2.prems"(3) irrefl, auto simp add: "2.prems"(1))
+    show "sorted_by {(x, y). R x y} (top_sort R (filter (R x) xs))"
+      by (rule 2, insert "2.prems"(3) irrefl, auto simp add: "2.prems"(1))
+    show "\<And>y. \<lbrakk>y \<in> set xs; R x y; R y x\<rbrakk> \<Longrightarrow> False"
+      using "2.prems"(2) "2.prems"(3) by auto
+    show "\<And>xa y. \<lbrakk>xa \<in> set xs; \<not> R x xa; y \<in> set xs; R x y; R y xa\<rbrakk> \<Longrightarrow> False"
+      by (smt "2.prems"(1) case_prodD case_prodI mem_Collect_eq transE)
+  qed
+qed
+
+lemma exists_sorted_by:
+  assumes fin: "finite S"
+    and trans: "trans R"
+    and irrefl2: "\<And>x y. x\<in>S \<Longrightarrow> y\<in>S \<Longrightarrow> (x,y)\<in>R \<Longrightarrow> x\<noteq>y \<Longrightarrow> (y,x)\<notin>R"
+shows "\<exists>l. set l = S \<and> sorted_by R l"
+proof -
+  obtain ul where "set ul = S" and "distinct ul"
+    using fin finite_distinct_list by auto
+
+  have "sorted_by R (top_sort (\<lambda>x y. (x,y)\<in>R) ul)"
+    by (fuzzy_rule top_sort_sorts_distinct; (simp add: trans `distinct ul`  \<open>set ul = S\<close> irrefl2)?)
+
+  thus ?thesis
+    by (metis \<open>set ul = S\<close> top_sort_set)
+qed
+
+lemma exists_sorted_by_irrefl:
+  assumes fin: "finite S"
+    and trans: "trans R"
+    and irrefl: "irrefl R"
+  shows "\<exists>l. set l = S \<and> sorted_by R l"
+  by (meson exists_sorted_by fin irrefl irrefl_def local.trans transE)
+
+lemma exists_sorted_by_antisym:
+  assumes fin: "finite S"
+    and trans: "trans R"
+    and irrefl: "antisym R"
+  shows "\<exists>l. set l = S \<and> sorted_by R l"
+  by (meson antisym_def exists_sorted_by fin irrefl local.trans)
+
+
+
+end
